theories/NormalIsomorphism.v
@@ -8,7 +8,7 @@ Import ListNotations.
 Definition irreducible s := ~exists s', Lambda.step s s'.
 
 (* In the text as claim 1. => *)
-Theorem nfs_are_irreducible :
+Proposition nfs_are_irreducible :
   (forall s, Lambda.normal s -> irreducible s)
   /\
   (forall s, apps s -> irreducible s).
@@ -17,14 +17,11 @@ Proof.
   - intro.
     apply H.
     destruct H0 as [s0 Hs0].
-    inversion Hs0.
-    now exists s'.
+    inversion Hs0. now exists s'.
     - intro.
       apply H.
-      destruct H0 as [s0 Hs0].
-      now exists s0.
-    - intro.
-      now destruct H.
+      destruct H0 as [s0 Hs0]. now exists s0.
+    - intro. now destruct H.
     - intro.
       destruct H1 as [s0 Hs0].
       inversion Hs0 ; subst.
@@ -34,7 +31,7 @@ Proof.
 Qed.
 
 (* In the text as claim 1. <= *)
-Theorem irreducible_is_nf s :
+Proposition irreducible_is_nf s :
   irreducible s -> Lambda.normal s.
 Proof.
   induction s ; intro H.
@@ -60,17 +57,68 @@ Proof.
       now exists (App s1 x).
 Qed.
 
-(* In the text as Claim 4. *)
-Definition irreducible' t := ~exists t', Canonical.step t t'.
-Conjecture nts_are_irreducible : forall t, Canonical.normal t -> irreducible' t.
-Conjecture irreducible_is_nt : forall t, irreducible' t -> Canonical.normal t.
+(* --- *)
+
+Definition can_irreducible t := ~exists t', Canonical.step t t'.
+Definition can_irreducible' l := ~exists l', Canonical.step' l l'.
+
+(* In the text as Claim 3. *)
+Proposition nts_are_irreducible :
+  (forall t, Canonical.normal t -> can_irreducible t)
+  /\
+  (forall l, Canonical.normal_list l -> can_irreducible' l).
+Proof.
+  apply Canonical.mut_normal_ind ; intros.
+  - intro H. destruct H as [u]. ainv.
+  - intro H'. destruct H' as [u]. inversion H0 ; subst.
+    + apply H. now exists t'.
+    + ainv.
+  - intro H'. destruct H' as [t']. inversion H1 ; subst.
+    + apply H. now exists u'.
+    + apply H0. now exists l'.
+    + ainv.
+  - intro H'. destruct H' as [l']. ainv.
+  - intro H'. destruct H' as [l']. inversion H1 ; subst.
+    + apply H. now exists u'.
+    + apply H0. now exists l'0.
+Qed.
+  
+Proposition irreducible_is_nt :
+  (forall t, can_irreducible t -> Canonical.normal t)
+  /\
+  (forall l, can_irreducible' l -> Canonical.normal_list l).
+Proof.
+  apply Canonical.mut_term_ind ; intros.
+  - constructor.
+  - constructor. apply H.
+    intro H'. destruct H' as [t'].
+    apply Comp_Lamb in H1. eauto.
+  - constructor.
+    + apply H.
+      intro H'. destruct H' as [u'].
+      apply Comp_VariApp1 with (x:=x) (l:=l) in H2. eauto.
+    + apply H0.
+      intro H'. destruct H' as [l'].
+      apply Comp_VariApp2 with (x:=x) (u:=u) in H2. eauto.
+  - destruct H2. destruct l.
+    + exists t.[u.:ids]. constructor. now left.
+    + exists (t.[u.:ids]@(t0, l)). constructor. now right.
+  - constructor.
+  - constructor.
+    + apply H. intro H'. destruct H' as [u'].
+      apply H1. eauto.
+    + apply H0. intro H'. destruct H' as [l'].
+      apply H1. eauto.      
+Qed.                      
+
+(* --- *)
 
 Corollary nf_inclusion s :
   Lambda.normal s -> Canonical.normal (ψ s).
 Proof.
   intro H.
   apply nfs_are_irreducible in H.
-  cut (irreducible' (ψ s)).
+  cut (can_irreducible (ψ s)).
   - apply irreducible_is_nt.
   - intro. apply H.
     inversion H0. apply θ_step_pres in H1.
