theories/Confluence.v
@@ -57,46 +57,45 @@ Qed.
 Require Import Lambda LambdaIsomorphism
   CanonicalIsomorphism Conservativeness.
 
-Section Confluence.
-  Hypothesis Lambda_confluence : forall s s1 s2,
-      Lambda.multistep s s1 -> Lambda.multistep s s2 ->
-      exists s', Lambda.multistep s1 s' /\ Lambda.multistep s2 s'.
+Theorem Lambda_confluence : forall s s1 s2,
+    Lambda.multistep s s1 -> Lambda.multistep s s2 ->
+    exists s', Lambda.multistep s1 s' /\ Lambda.multistep s2 s'.
+Admitted.
 
-  Corollary Canonical_confluence : forall t t1 t2,
-      Canonical.multistep t t1 -> Canonical.multistep t t2 ->
-      exists t', Canonical.multistep t1 t' /\ Canonical.multistep t2 t'.
-  Proof.
-    intros t t1 t2 Htt1 Htt2.
-    apply θ_multistep_pres in Htt1.
-    apply θ_multistep_pres in Htt2.
-    specialize (Lambda_confluence _ _ _ Htt1 Htt2) as (s & H1s & H2s).
-    exists (ψ s). split.
-    - apply ψ_multistep_pres in H1s.
-      now rewrite (proj1 LambdaIsomorphism.inversion1) in H1s.
-    - apply ψ_multistep_pres in H2s.
-      now rewrite (proj1 LambdaIsomorphism.inversion1) in H2s.
-  Qed.
+Corollary Canonical_confluence : forall t t1 t2,
+    Canonical.multistep t t1 -> Canonical.multistep t t2 ->
+    exists t', Canonical.multistep t1 t' /\ Canonical.multistep t2 t'.
+Proof.
+  intros t t1 t2 Htt1 Htt2.
+  apply θ_multistep_pres in Htt1.
+  apply θ_multistep_pres in Htt2.
+  specialize (Lambda_confluence _ _ _ Htt1 Htt2) as (s & H1s & H2s).
+  exists (ψ s). split.
+  - apply ψ_multistep_pres in H1s.
+    now rewrite (proj1 LambdaIsomorphism.inversion1) in H1s.
+  - apply ψ_multistep_pres in H2s.
+    now rewrite (proj1 LambdaIsomorphism.inversion1) in H2s.
+Qed.
 
-  Corollary LambdaM_confluence : forall t t1 t2,
+Corollary LambdaM_confluence : forall t t1 t2,
     LambdaM.multistep t t1 -> LambdaM.multistep t t2 ->
     exists t', LambdaM.multistep t1 t' /\ LambdaM.multistep t2 t'.
-  Proof.
-    intros t t1 t2 Htt1 Htt2.
-    apply conservativeness2' in Htt1.
-    apply conservativeness2' in Htt2.
-    specialize (Canonical_confluence _ _ _ Htt1 Htt2) as (t' & H1 & H2).
-    exists (i t'). split.
-    - apply conservativeness in H1.
-      rewrite (proj1 inversion1) in H1.
-      apply multistep_trans with (h t1).
-      + apply multistep_H_inclusion.
-        apply h_is_multistep_H.
-      + assumption.
-    - apply conservativeness in H2.
-      rewrite (proj1 inversion1) in H2.
-      apply multistep_trans with (h t2).
-      + apply multistep_H_inclusion.
-        apply h_is_multistep_H.
-      + assumption.
-  Qed.
-End Confluence.
+Proof.
+  intros t t1 t2 Htt1 Htt2.
+  apply conservativeness2' in Htt1.
+  apply conservativeness2' in Htt2.
+  specialize (Canonical_confluence _ _ _ Htt1 Htt2) as (t' & H1 & H2).
+  exists (i t'). split.
+  - apply conservativeness in H1.
+    rewrite (proj1 inversion1) in H1.
+    apply multistep_trans with (h t1).
+    + apply multistep_H_inclusion.
+      apply h_is_multistep_H.
+    + assumption.
+  - apply conservativeness in H2.
+    rewrite (proj1 inversion1) in H2.
+    apply multistep_trans with (h t2).
+    + apply multistep_H_inclusion.
+      apply h_is_multistep_H.
+    + assumption.
+Qed.
